Clean up: more splitting into files

OptSim.v
@@ -33,13 +33,13 @@ End SimOpt.
 Section WithLTS.
 
 Context {lts : LTS}.
-Let Observable := lts.(Observable).
-Let St := lts.(St).
-Let trans := lts.(trans).
-Let epsilon := lts.(epsilon).
-Let Robs := lts.(Robs).
-Let ub_state := lts.(ub_state).
-Let label := @label Observable.
+Notation Observable := lts.(Observable).
+Notation St := lts.(St).
+Notation trans := lts.(trans).
+Notation epsilon := lts.(epsilon).
+Notation Robs := lts.(Robs).
+Notation ub_state := lts.(ub_state).
+Notation label := (@label Observable).
 
 Section SimDef.
 
@@ -272,47 +272,6 @@ Proof.
   - apply (gfp_fp simF). now constructor.
 Qed.
 
-Program Definition divsimF lock : mon (St -> St -> Prop) :=
-{|
-  body := fun R s t => (forall o s', ((trans tau)^* ⋅ trans (obs o)) s s' ->
-    exists o' t',
-        ((trans tau)^* ⋅ trans (obs o')) t t' /\
-      R s' t' /\
-      Robs o o') /\
-  (forall s', (trans tau)^* s s' ->
-    exists t', 
-      (trans tau)^* t t' /\ R s' t') /\
-  (diverges s -> diverges t) /\
-  (lock = SimOpt.nolock \/ (is_stuck s -> is_stuck t))
-|}.
-Next Obligation.
-  repeat split; intros; auto.
-  - apply H0 in H4 as (? & ? & ? & ? & ?). eauto 6.
-  - apply H1 in H4 as (? & ? & ?). eauto.
-Qed.
-
-Definition divsim := gfp (divsimF SimOpt.nolock).
-
-Program Definition divsimF' : mon (St -> St -> Prop) :=
-{|
-  body := fun R s t => (forall o s', trans (obs o) s s' ->
-    exists o' t',
-        ((trans tau)^* ⋅ trans (obs o')) t t' /\
-      R s' t' /\
-      Robs o o') /\
-  (forall s', trans tau s s' ->
-    exists t', 
-      (trans tau)^* t t' /\ R s' t') /\
-  (diverges s -> diverges t)
-|}.
-Next Obligation.
-  repeat split; intros; auto.
-  - apply H0 in H3 as (? & ? & ? & ? & ?). eauto 6.
-  - apply H1 in H3 as (? & ? & ?). eauto.
-Qed.
-
-Definition divsim' := gfp divsimF'.
-
 Lemma chain_div : forall (R : Chain simF) s t,
   diverges t ->
   simF `R false s t.
@@ -346,43 +305,6 @@ Lemma trans_add_delay : forall l,
 Proof.
   intros. esplit; eauto. now rewrite <- str_refl.
 Qed.
-
-Lemma divsim_divpres : forall s t,
-  divsim s t ->
-  sim false s t.
-Proof.
-  red. coinduction R CH. intros.
-  apply (gfp_fp (divsimF _)) in H. destruct H as (_ & _ & ? & _).
-  destruct (diverges_lem s).
-  apply H in H0. eapply chain_div in H0. apply H0; auto.
-  eapply chain_nodiv with (R := R) (t := t) in H0. apply H0; auto.
-Qed.
-
-(* ok *)
-Lemma divsim_equiv
-  (Hfreeze : freeze = SimOpt.freeze_div)
-  (Hlock : lock = SimOpt.nolock)
-  (Hdelay : delay = SimOpt.delay) :
-  forall b s t, divsim s t ->
-  sim b s t.
-Proof.
-  red. coinduction R CH. intros. destruct b.
-  2: now apply (gfp_bchain R), divsim_divpres.
-  constructor.
-  repeat split; intros.
-  - apply (gfp_fp (divsimF _)) in H. destruct H as (? & ? & _).
-    apply trans_add_delay in H0.
-    apply H in H0 as (? & ? & ? & ? & ?).
-    eapply ans_delay_obs; eauto.
-  - apply (gfp_fp (divsimF _)) in H.
-    rewrite (str_ext (trans tau)) in H0.
-    apply H in H0 as (? & ? & ?).
-    rewrite str_itr in H0. destruct H0.
-    + apply tau_div. assumption. apply CH. cbn in H0. admit.
-      apply CH. admit.
-    + eapply tau_delay; eauto.
-  - now left.
-Admitted.
 
 Lemma divpresF_tau_r : forall (R : Chain simF) s t t',
   `R false s t' ->
@@ -441,34 +363,6 @@ Proof.
   revert s t H. apply gfp_prop.
   intros. apply simF_f_t; auto.
   now rewrite Hfreeze.
-Qed.
-
-Lemma divsim_equiv'
-  (Hfreeze : freeze = SimOpt.freeze_div)
-  (Hlock : lock = SimOpt.nolock)
-  (Hdelay : delay = SimOpt.delay) :
-  forall s t, (forall b, sim b s t) ->
-  divsim' s t.
-Proof.
-  red. coinduction R CH. intros. cbn -[dot str]. repeat split; intros.
-  - specialize (H true). apply sim_fp in H. apply H in H0 as []; auto.
-    + exists o', t'. split. { now apply trans_add_delay. }
-      split; auto. apply CH. intros. destruct b; auto.
-      now apply sim_f_t.
-    + exists o', t'. repeat split; auto.
-      apply CH. intros. destruct b; auto. now apply sim_f_t.
-  - specialize (H true). apply sim_fp in H. apply H in H0 as []; auto.
-    + exists t'. split. { now rewrite <- str_ext. }
-      apply CH. intros []; auto. now apply sim_f_t.
-    + now rewrite Hfreeze in H0.
-    + exists t. split. { now rewrite <- str_refl. }
-      apply CH. intros []; try easy.
-    + exists t'. split. { now rewrite <- str_itr'. }
-      apply CH. intros []; auto. now apply sim_f_t.
-  - specialize (H false). revert s t H H0. clear R CH. red. coinduction R CH. intros.
-    cbn. apply sim_fp in H. revert H0. induction H. intros.
-    apply (gfp_fp divergesF) in H0 as (? & ? & ?). apply H in H0. destruct H0; eauto.
-    destruct DIV. apply H2 in H1 as (? & ? & ?). eauto.
 Qed.
 
 Lemma sim_tau_l (R : Chain simF) (Hfreeze : freeze = SimOpt.freeze_div) :
