DivSim.v
@@ -1,0 +1,138 @@
+From Coinduction Require Import all.
+From RelationAlgebra Require Import
+     kat
+     kat_tac
+     prop
+     rel
+     srel
+     comparisons
+     rewriting
+     normalisation
+     monoid.
+From OptSim Require Import Utils LTS Divergence OptSim.
+
+Section WithLTS.
+
+Context {lts : LTS}.
+
+Notation Observable := lts.(Observable).
+Notation St := lts.(St).
+Notation trans := lts.(trans).
+Notation epsilon := lts.(epsilon).
+Notation Robs := lts.(Robs).
+Notation ub_state := lts.(ub_state).
+Notation label := (@label Observable).
+
+Program Definition divsimF lock : mon (St -> St -> Prop) :=
+{|
+  body := fun R s t => (forall o s', ((trans tau)^* ⋅ trans (obs o)) s s' ->
+    exists o' t',
+        ((trans tau)^* ⋅ trans (obs o')) t t' /\
+      R s' t' /\
+      Robs o o') /\
+  (forall s', (trans tau)^* s s' ->
+    exists t', 
+      (trans tau)^* t t' /\ R s' t') /\
+  (diverges s -> diverges t) /\
+  (lock = SimOpt.nolock \/ (is_stuck s -> is_stuck t))
+|}.
+Next Obligation.
+  repeat split; intros; auto.
+  - apply H0 in H4 as (? & ? & ? & ? & ?). eauto 6.
+  - apply H1 in H4 as (? & ? & ?). eauto.
+Qed.
+
+Definition divsim := gfp (divsimF SimOpt.nolock).
+
+Program Definition divsimF' : mon (St -> St -> Prop) :=
+{|
+  body := fun R s t => (forall o s', trans (obs o) s s' ->
+    exists o' t',
+        ((trans tau)^* ⋅ trans (obs o')) t t' /\
+      R s' t' /\
+      Robs o o') /\
+  (forall s', trans tau s s' ->
+    exists t', 
+      (trans tau)^* t t' /\ R s' t') /\
+  (diverges s -> diverges t)
+|}.
+Next Obligation.
+  repeat split; intros; auto.
+  - apply H0 in H3 as (? & ? & ? & ? & ?). eauto 6.
+  - apply H1 in H3 as (? & ? & ?). eauto.
+Qed.
+
+Definition divsim' := gfp divsimF'.
+
+Section WithOpts.
+
+Context (freeze : SimOpt.freeze_opt)
+  (lock : SimOpt.lock_opt) (delay : SimOpt.delay_opt).
+
+Lemma divsim_divpres : forall s t,
+  divsim s t ->
+  sim freeze lock delay false s t.
+Proof.
+  red. coinduction R CH. intros.
+  apply (gfp_fp (divsimF _)) in H. destruct H as (_ & _ & ? & _).
+  destruct (diverges_lem s).
+  apply H in H0. eapply chain_div in H0. apply H0; auto.
+  eapply chain_nodiv with (R := R) (t := t) in H0. apply H0; auto.
+Qed.
+
+(* ok *)
+Lemma divsim_equiv
+  (Hfreeze : freeze = SimOpt.freeze_div)
+  (Hlock : lock = SimOpt.nolock)
+  (Hdelay : delay = SimOpt.delay) :
+  forall b s t, divsim s t ->
+  sim freeze lock delay b s t.
+Proof.
+  red. coinduction R CH. intros. destruct b.
+  2: now apply (gfp_bchain R), divsim_divpres.
+  constructor.
+  repeat split; intros.
+  - apply (gfp_fp (divsimF _)) in H. destruct H as (? & ? & _).
+    apply trans_add_delay in H0.
+    apply H in H0 as (? & ? & ? & ? & ?).
+    eapply ans_delay_obs; eauto.
+  - apply (gfp_fp (divsimF _)) in H.
+    rewrite (str_ext (trans tau)) in H0.
+    apply H in H0 as (? & ? & ?).
+    rewrite str_itr in H0. destruct H0.
+    + apply tau_div. assumption. apply CH. cbn in H0. admit.
+      apply CH. admit.
+    + eapply tau_delay; eauto.
+  - now left.
+Admitted.
+
+Lemma divsim_equiv'
+  (Hfreeze : freeze = SimOpt.freeze_div)
+  (Hlock : lock = SimOpt.nolock)
+  (Hdelay : delay = SimOpt.delay) :
+  forall s t, (forall b, sim freeze lock delay b s t) ->
+  divsim' s t.
+Proof.
+  red. coinduction R CH. intros. cbn -[dot str]. repeat split; intros.
+  - specialize (H true). apply sim_fp in H. apply H in H0 as []; auto.
+    + exists o', t'. split. { now apply trans_add_delay. }
+      split; auto. apply CH. intros. destruct b; auto.
+      now apply sim_f_t.
+    + exists o', t'. repeat split; auto.
+      apply CH. intros. destruct b; auto. now apply sim_f_t.
+  - specialize (H true). apply sim_fp in H. apply H in H0 as []; auto.
+    + exists t'. split. { now rewrite <- str_ext. }
+      apply CH. intros []; auto. now apply sim_f_t.
+    + now rewrite Hfreeze in H0.
+    + exists t. split. { now rewrite <- str_refl. }
+      apply CH. intros []; try easy.
+    + exists t'. split. { now rewrite <- str_itr'. }
+      apply CH. intros []; auto. now apply sim_f_t.
+  - specialize (H false). revert s t H H0. clear R CH. red. coinduction R CH. intros.
+    cbn. apply sim_fp in H. revert H0. induction H. intros.
+    apply (gfp_fp divergesF) in H0 as (? & ? & ?). apply H in H0. destruct H0; eauto.
+    destruct DIV. apply H2 in H1 as (? & ? & ?). eauto.
+Qed.
+
+End WithOpts.
+End WithLTS.
