Divergence.v
@@ -17,13 +17,13 @@ Import CoindNotations.
 Section WithLTS.
 
 Context {lts : LTS}.
-Let Observable := lts.(Observable).
-Let St := lts.(St).
-Let trans := lts.(trans).
-Let epsilon := lts.(epsilon).
-Let Robs := lts.(Robs).
-Let ub_state := lts.(ub_state).
-Let label := @label Observable.
+Notation Observable := lts.(Observable).
+Notation St := lts.(St).
+Notation trans := lts.(trans).
+Notation epsilon := lts.(epsilon).
+Notation Robs := lts.(Robs).
+Notation ub_state := lts.(ub_state).
+Notation label := (@label Observable).
 
 Program Definition divergesF : mon (St -> Prop) :=
 {| body R st :=
